Updates from CodeGen

src/AwsCryptographicMaterialProviders/Model/AwsCryptographyMaterialProvidersTypes.dfy
@@ -30,215 +30,300 @@ include "../../StandardLibrary/StandardLibrary.dfy"
 	| ALG_AES_256_GCM_IV12_TAG16_HKDF_SHA384_ECDSA_P384
 	| ALG_AES_256_GCM_HKDF_SHA512_COMMIT_KEY
 	| ALG_AES_256_GCM_HKDF_SHA512_COMMIT_KEY_ECDSA_P384
- datatype AlgorithmSuiteInfo = AlgorithmSuiteInfo ( nameonly id: AlgorithmSuiteId ,
+ datatype AlgorithmSuiteInfo = | AlgorithmSuiteInfo (
+ nameonly id: AlgorithmSuiteId ,
  nameonly encrypt: AwsCryptographyPrimitivesTypes.AES_GCM ,
- nameonly kdf: DerivationAlgorithm )
- trait {:termination false} IAwsCryptographicMaterialProvidersClient {
- predicate {:opaque} CreateAwsKmsKeyringCalledWith ( input: CreateAwsKmsKeyringInput ) {true}
- predicate {:opaque} CreateAwsKmsKeyringSucceededWith (  input: CreateAwsKmsKeyringInput , output: IKeyring ) {true}
- method CreateAwsKmsKeyring ( input: CreateAwsKmsKeyringInput ) returns  ( output: Result<IKeyring, Error> )
+ nameonly kdf: DerivationAlgorithm ,
+ nameonly commitment: DerivationAlgorithm ,
+ nameonly signature: SignatureAlgorithm
+ )
+ trait {:termination false} IAwsCryptographicMaterialProvidersClient
+ {
+ method CreateAwsKmsKeyring ( input: CreateAwsKmsKeyringInput ) returns (output: Result<IKeyring, Error>)
 	ensures CreateAwsKmsKeyringCalledWith (  input )
 	ensures output.Success? ==> CreateAwsKmsKeyringSucceededWith (  input , output.value )
-
- predicate {:opaque} CreateAwsKmsDiscoveryKeyringCalledWith ( input: CreateAwsKmsDiscoveryKeyringInput ) {true}
- predicate {:opaque} CreateAwsKmsDiscoveryKeyringSucceededWith (  input: CreateAwsKmsDiscoveryKeyringInput , output: IKeyring ) {true}
- method CreateAwsKmsDiscoveryKeyring ( input: CreateAwsKmsDiscoveryKeyringInput ) returns  ( output: Result<IKeyring, Error> )
+ method CreateAwsKmsDiscoveryKeyring ( input: CreateAwsKmsDiscoveryKeyringInput ) returns (output: Result<IKeyring, Error>)
 	ensures CreateAwsKmsDiscoveryKeyringCalledWith (  input )
 	ensures output.Success? ==> CreateAwsKmsDiscoveryKeyringSucceededWith (  input , output.value )
-
- predicate {:opaque} CreateAwsKmsMultiKeyringCalledWith ( input: CreateAwsKmsMultiKeyringInput ) {true}
- predicate {:opaque} CreateAwsKmsMultiKeyringSucceededWith (  input: CreateAwsKmsMultiKeyringInput , output: IKeyring ) {true}
- method CreateAwsKmsMultiKeyring ( input: CreateAwsKmsMultiKeyringInput ) returns  ( output: Result<IKeyring, Error> )
+ method CreateAwsKmsMultiKeyring ( input: CreateAwsKmsMultiKeyringInput ) returns (output: Result<IKeyring, Error>)
 	ensures CreateAwsKmsMultiKeyringCalledWith (  input )
 	ensures output.Success? ==> CreateAwsKmsMultiKeyringSucceededWith (  input , output.value )
-
- predicate {:opaque} CreateAwsKmsDiscoveryMultiKeyringCalledWith ( input: CreateAwsKmsDiscoveryMultiKeyringInput ) {true}
- predicate {:opaque} CreateAwsKmsDiscoveryMultiKeyringSucceededWith (  input: CreateAwsKmsDiscoveryMultiKeyringInput , output: IKeyring ) {true}
- method CreateAwsKmsDiscoveryMultiKeyring ( input: CreateAwsKmsDiscoveryMultiKeyringInput ) returns  ( output: Result<IKeyring, Error> )
+ method CreateAwsKmsDiscoveryMultiKeyring ( input: CreateAwsKmsDiscoveryMultiKeyringInput ) returns (output: Result<IKeyring, Error>)
 	ensures CreateAwsKmsDiscoveryMultiKeyringCalledWith (  input )
 	ensures output.Success? ==> CreateAwsKmsDiscoveryMultiKeyringSucceededWith (  input , output.value )
-
- predicate {:opaque} CreateAwsKmsMrkKeyringCalledWith ( input: CreateAwsKmsMrkKeyringInput ) {true}
- predicate {:opaque} CreateAwsKmsMrkKeyringSucceededWith (  input: CreateAwsKmsMrkKeyringInput , output: IKeyring ) {true}
- method CreateAwsKmsMrkKeyring ( input: CreateAwsKmsMrkKeyringInput ) returns  ( output: Result<IKeyring, Error> )
+ method CreateAwsKmsMrkKeyring ( input: CreateAwsKmsMrkKeyringInput ) returns (output: Result<IKeyring, Error>)
 	ensures CreateAwsKmsMrkKeyringCalledWith (  input )
 	ensures output.Success? ==> CreateAwsKmsMrkKeyringSucceededWith (  input , output.value )
-
- predicate {:opaque} CreateAwsKmsMrkMultiKeyringCalledWith ( input: CreateAwsKmsMrkMultiKeyringInput ) {true}
- predicate {:opaque} CreateAwsKmsMrkMultiKeyringSucceededWith (  input: CreateAwsKmsMrkMultiKeyringInput , output: IKeyring ) {true}
- method CreateAwsKmsMrkMultiKeyring ( input: CreateAwsKmsMrkMultiKeyringInput ) returns  ( output: Result<IKeyring, Error> )
+ method CreateAwsKmsMrkMultiKeyring ( input: CreateAwsKmsMrkMultiKeyringInput ) returns (output: Result<IKeyring, Error>)
 	ensures CreateAwsKmsMrkMultiKeyringCalledWith (  input )
 	ensures output.Success? ==> CreateAwsKmsMrkMultiKeyringSucceededWith (  input , output.value )
-
- predicate {:opaque} CreateAwsKmsMrkDiscoveryKeyringCalledWith ( input: CreateAwsKmsMrkDiscoveryKeyringInput ) {true}
- predicate {:opaque} CreateAwsKmsMrkDiscoveryKeyringSucceededWith (  input: CreateAwsKmsMrkDiscoveryKeyringInput , output: IKeyring ) {true}
- method CreateAwsKmsMrkDiscoveryKeyring ( input: CreateAwsKmsMrkDiscoveryKeyringInput ) returns  ( output: Result<IKeyring, Error> )
+ method CreateAwsKmsMrkDiscoveryKeyring ( input: CreateAwsKmsMrkDiscoveryKeyringInput ) returns (output: Result<IKeyring, Error>)
 	ensures CreateAwsKmsMrkDiscoveryKeyringCalledWith (  input )
 	ensures output.Success? ==> CreateAwsKmsMrkDiscoveryKeyringSucceededWith (  input , output.value )
-
- predicate {:opaque} CreateAwsKmsMrkDiscoveryMultiKeyringCalledWith ( input: CreateAwsKmsMrkDiscoveryMultiKeyringInput ) {true}
- predicate {:opaque} CreateAwsKmsMrkDiscoveryMultiKeyringSucceededWith (  input: CreateAwsKmsMrkDiscoveryMultiKeyringInput , output: IKeyring ) {true}
- method CreateAwsKmsMrkDiscoveryMultiKeyring ( input: CreateAwsKmsMrkDiscoveryMultiKeyringInput ) returns  ( output: Result<IKeyring, Error> )
+ method CreateAwsKmsMrkDiscoveryMultiKeyring ( input: CreateAwsKmsMrkDiscoveryMultiKeyringInput ) returns (output: Result<IKeyring, Error>)
 	ensures CreateAwsKmsMrkDiscoveryMultiKeyringCalledWith (  input )
 	ensures output.Success? ==> CreateAwsKmsMrkDiscoveryMultiKeyringSucceededWith (  input , output.value )
-
- predicate {:opaque} CreateMultiKeyringCalledWith ( input: CreateMultiKeyringInput ) {true}
- predicate {:opaque} CreateMultiKeyringSucceededWith (  input: CreateMultiKeyringInput , output: IKeyring ) {true}
- method CreateMultiKeyring ( input: CreateMultiKeyringInput ) returns  ( output: Result<IKeyring, Error> )
+ method CreateMultiKeyring ( input: CreateMultiKeyringInput ) returns (output: Result<IKeyring, Error>)
 	ensures CreateMultiKeyringCalledWith (  input )
 	ensures output.Success? ==> CreateMultiKeyringSucceededWith (  input , output.value )
-
- predicate {:opaque} CreateRawAesKeyringCalledWith ( input: CreateRawAesKeyringInput ) {true}
- predicate {:opaque} CreateRawAesKeyringSucceededWith (  input: CreateRawAesKeyringInput , output: IKeyring ) {true}
- method CreateRawAesKeyring ( input: CreateRawAesKeyringInput ) returns  ( output: Result<IKeyring, Error> )
+ method CreateRawAesKeyring ( input: CreateRawAesKeyringInput ) returns (output: Result<IKeyring, Error>)
 	ensures CreateRawAesKeyringCalledWith (  input )
 	ensures output.Success? ==> CreateRawAesKeyringSucceededWith (  input , output.value )
-
- predicate {:opaque} CreateRawRsaKeyringCalledWith ( input: CreateRawRsaKeyringInput ) {true}
- predicate {:opaque} CreateRawRsaKeyringSucceededWith (  input: CreateRawRsaKeyringInput , output: IKeyring ) {true}
- method CreateRawRsaKeyring ( input: CreateRawRsaKeyringInput ) returns  ( output: Result<IKeyring, Error> )
+ method CreateRawRsaKeyring ( input: CreateRawRsaKeyringInput ) returns (output: Result<IKeyring, Error>)
 	ensures CreateRawRsaKeyringCalledWith (  input )
 	ensures output.Success? ==> CreateRawRsaKeyringSucceededWith (  input , output.value )
-
- predicate {:opaque} CreateDefaultCryptographicMaterialsManagerCalledWith ( input: CreateDefaultCryptographicMaterialsManagerInput ) {true}
- predicate {:opaque} CreateDefaultCryptographicMaterialsManagerSucceededWith (  input: CreateDefaultCryptographicMaterialsManagerInput , output: ICryptographicMaterialsManager ) {true}
- method CreateDefaultCryptographicMaterialsManager ( input: CreateDefaultCryptographicMaterialsManagerInput ) returns  ( output: Result<ICryptographicMaterialsManager, Error> )
+ method CreateDefaultCryptographicMaterialsManager ( input: CreateDefaultCryptographicMaterialsManagerInput ) returns (output: Result<ICryptographicMaterialsManager, Error>)
 	ensures CreateDefaultCryptographicMaterialsManagerCalledWith (  input )
 	ensures output.Success? ==> CreateDefaultCryptographicMaterialsManagerSucceededWith (  input , output.value )
-
- predicate {:opaque} CreateDefaultClientSupplierCalledWith ( input: CreateDefaultClientSupplierInput ) {true}
- predicate {:opaque} CreateDefaultClientSupplierSucceededWith (  input: CreateDefaultClientSupplierInput , output: IClientSupplier ) {true}
- method CreateDefaultClientSupplier ( input: CreateDefaultClientSupplierInput ) returns  ( output: Result<IClientSupplier, Error> )
+ method CreateDefaultClientSupplier ( input: CreateDefaultClientSupplierInput ) returns (output: Result<IClientSupplier, Error>)
 	ensures CreateDefaultClientSupplierCalledWith (  input )
 	ensures output.Success? ==> CreateDefaultClientSupplierSucceededWith (  input , output.value )
-
+ method InitializeEncryptionMaterials ( input: InitializeMaterialsInput ) returns (output: Result<EncryptionMaterials, Error>)
+	ensures InitializeEncryptionMaterialsCalledWith (  input )
+	ensures output.Success? ==> InitializeEncryptionMaterialsSucceededWith (  input , output.value )
+ method InitializeDecryptionMaterials ( input: InitializeMaterialsInput ) returns (output: Result<DecryptionMaterials, Error>)
+	ensures InitializeDecryptionMaterialsCalledWith (  input )
+	ensures output.Success? ==> InitializeDecryptionMaterialsSucceededWith (  input , output.value )
+ method ValidEncryptionMaterialsTransition ( input: ValidEncryptionMaterialsTransitionInput ) returns (output: Result<bool, Error>)
+	ensures ValidEncryptionMaterialsTransitionCalledWith (  input )
+	ensures output.Success? ==> ValidEncryptionMaterialsTransitionSucceededWith (  input , output.value )
+ method ValidDecryptionMaterialsTransition ( input: ValidDecryptionMaterialsTransitionInput ) returns (output: Result<bool, Error>)
+	ensures ValidDecryptionMaterialsTransitionCalledWith (  input )
+	ensures output.Success? ==> ValidDecryptionMaterialsTransitionSucceededWith (  input , output.value )
 }
- trait {:termination false} IClientSupplier {
- predicate {:opaque} GetClientCalledWith ( input: GetClientInput ) {true}
- predicate {:opaque} GetClientSucceededWith (  input: GetClientInput , output: ComAmazonawsKmsTypes.IKeyManagementServiceClient ) {true}
- method GetClient ( input: GetClientInput ) returns  ( output: Result<ComAmazonawsKmsTypes.IKeyManagementServiceClient, Error> )
+ // Predicates are separated from the trait. This is temporary.
+ predicate {:opaque} CreateAwsKmsKeyringCalledWith ( input: CreateAwsKmsKeyringInput ) {true}
+ predicate {:opaque} CreateAwsKmsKeyringSucceededWith (  input: CreateAwsKmsKeyringInput , output: IKeyring ) {true}
+ predicate {:opaque} CreateAwsKmsDiscoveryKeyringCalledWith ( input: CreateAwsKmsDiscoveryKeyringInput ) {true}
+ predicate {:opaque} CreateAwsKmsDiscoveryKeyringSucceededWith (  input: CreateAwsKmsDiscoveryKeyringInput , output: IKeyring ) {true}
+ predicate {:opaque} CreateAwsKmsMultiKeyringCalledWith ( input: CreateAwsKmsMultiKeyringInput ) {true}
+ predicate {:opaque} CreateAwsKmsMultiKeyringSucceededWith (  input: CreateAwsKmsMultiKeyringInput , output: IKeyring ) {true}
+ predicate {:opaque} CreateAwsKmsDiscoveryMultiKeyringCalledWith ( input: CreateAwsKmsDiscoveryMultiKeyringInput ) {true}
+ predicate {:opaque} CreateAwsKmsDiscoveryMultiKeyringSucceededWith (  input: CreateAwsKmsDiscoveryMultiKeyringInput , output: IKeyring ) {true}
+ predicate {:opaque} CreateAwsKmsMrkKeyringCalledWith ( input: CreateAwsKmsMrkKeyringInput ) {true}
+ predicate {:opaque} CreateAwsKmsMrkKeyringSucceededWith (  input: CreateAwsKmsMrkKeyringInput , output: IKeyring ) {true}
+ predicate {:opaque} CreateAwsKmsMrkMultiKeyringCalledWith ( input: CreateAwsKmsMrkMultiKeyringInput ) {true}
+ predicate {:opaque} CreateAwsKmsMrkMultiKeyringSucceededWith (  input: CreateAwsKmsMrkMultiKeyringInput , output: IKeyring ) {true}
+ predicate {:opaque} CreateAwsKmsMrkDiscoveryKeyringCalledWith ( input: CreateAwsKmsMrkDiscoveryKeyringInput ) {true}
+ predicate {:opaque} CreateAwsKmsMrkDiscoveryKeyringSucceededWith (  input: CreateAwsKmsMrkDiscoveryKeyringInput , output: IKeyring ) {true}
+ predicate {:opaque} CreateAwsKmsMrkDiscoveryMultiKeyringCalledWith ( input: CreateAwsKmsMrkDiscoveryMultiKeyringInput ) {true}
+ predicate {:opaque} CreateAwsKmsMrkDiscoveryMultiKeyringSucceededWith (  input: CreateAwsKmsMrkDiscoveryMultiKeyringInput , output: IKeyring ) {true}
+ predicate {:opaque} CreateMultiKeyringCalledWith ( input: CreateMultiKeyringInput ) {true}
+ predicate {:opaque} CreateMultiKeyringSucceededWith (  input: CreateMultiKeyringInput , output: IKeyring ) {true}
+ predicate {:opaque} CreateRawAesKeyringCalledWith ( input: CreateRawAesKeyringInput ) {true}
+ predicate {:opaque} CreateRawAesKeyringSucceededWith (  input: CreateRawAesKeyringInput , output: IKeyring ) {true}
+ predicate {:opaque} CreateRawRsaKeyringCalledWith ( input: CreateRawRsaKeyringInput ) {true}
+ predicate {:opaque} CreateRawRsaKeyringSucceededWith (  input: CreateRawRsaKeyringInput , output: IKeyring ) {true}
+ predicate {:opaque} CreateDefaultCryptographicMaterialsManagerCalledWith ( input: CreateDefaultCryptographicMaterialsManagerInput ) {true}
+ predicate {:opaque} CreateDefaultCryptographicMaterialsManagerSucceededWith (  input: CreateDefaultCryptographicMaterialsManagerInput , output: ICryptographicMaterialsManager ) {true}
+ predicate {:opaque} CreateDefaultClientSupplierCalledWith ( input: CreateDefaultClientSupplierInput ) {true}
+ predicate {:opaque} CreateDefaultClientSupplierSucceededWith (  input: CreateDefaultClientSupplierInput , output: IClientSupplier ) {true}
+ predicate {:opaque} InitializeEncryptionMaterialsCalledWith ( input: InitializeMaterialsInput ) {true}
+ predicate {:opaque} InitializeEncryptionMaterialsSucceededWith (  input: InitializeMaterialsInput , output: EncryptionMaterials ) {true}
+ predicate {:opaque} InitializeDecryptionMaterialsCalledWith ( input: InitializeMaterialsInput ) {true}
+ predicate {:opaque} InitializeDecryptionMaterialsSucceededWith (  input: InitializeMaterialsInput , output: DecryptionMaterials ) {true}
+ predicate {:opaque} ValidEncryptionMaterialsTransitionCalledWith ( input: ValidEncryptionMaterialsTransitionInput ) {true}
+ predicate {:opaque} ValidEncryptionMaterialsTransitionSucceededWith (  input: ValidEncryptionMaterialsTransitionInput , output: bool ) {true}
+ predicate {:opaque} ValidDecryptionMaterialsTransitionCalledWith ( input: ValidDecryptionMaterialsTransitionInput ) {true}
+ predicate {:opaque} ValidDecryptionMaterialsTransitionSucceededWith (  input: ValidDecryptionMaterialsTransitionInput , output: bool ) {true}
+ trait {:termination false} IClientSupplier
+ {
+ method GetClient ( input: GetClientInput ) returns (output: Result<ComAmazonawsKmsTypes.IKeyManagementServiceClient, Error>)
 	ensures GetClientCalledWith (  input )
 	ensures output.Success? ==> GetClientSucceededWith (  input , output.value )
-
 }
+ // Predicates are separated from the trait. This is temporary.
+ predicate {:opaque} GetClientCalledWith ( input: GetClientInput ) {true}
+ predicate {:opaque} GetClientSucceededWith (  input: GetClientInput , output: ComAmazonawsKmsTypes.IKeyManagementServiceClient ) {true}
  datatype CommitmentPolicy =
 	| FORBID_ENCRYPT_ALLOW_DECRYPT
 	| REQUIRE_ENCRYPT_ALLOW_DECRYPT
 	| REQUIRE_ENCRYPT_REQUIRE_DECRYPT
- datatype CreateAwsKmsDiscoveryKeyringInput = CreateAwsKmsDiscoveryKeyringInput ( nameonly kmsClient: ComAmazonawsKmsTypes.IKeyManagementServiceClient ,
+ datatype CreateAwsKmsDiscoveryKeyringInput = | CreateAwsKmsDiscoveryKeyringInput (
+ nameonly kmsClient: ComAmazonawsKmsTypes.IKeyManagementServiceClient ,
  nameonly discoveryFilter: Option<DiscoveryFilter> ,
- nameonly grantTokens: Option<GrantTokenList> )
- datatype CreateAwsKmsDiscoveryMultiKeyringInput = CreateAwsKmsDiscoveryMultiKeyringInput ( nameonly regions: RegionList ,
+ nameonly grantTokens: Option<GrantTokenList>
+ )
+ datatype CreateAwsKmsDiscoveryMultiKeyringInput = | CreateAwsKmsDiscoveryMultiKeyringInput (
+ nameonly regions: RegionList ,
  nameonly discoveryFilter: Option<DiscoveryFilter> ,
  nameonly clientSupplier: Option<IClientSupplier> ,
- nameonly grantTokens: Option<GrantTokenList> )
- datatype CreateAwsKmsKeyringInput = CreateAwsKmsKeyringInput ( nameonly kmsKeyId: KmsKeyId ,
+ nameonly grantTokens: Option<GrantTokenList>
+ )
+ datatype CreateAwsKmsKeyringInput = | CreateAwsKmsKeyringInput (
+ nameonly kmsKeyId: KmsKeyId ,
  nameonly kmsClient: ComAmazonawsKmsTypes.IKeyManagementServiceClient ,
- nameonly grantTokens: Option<GrantTokenList> )
- datatype CreateAwsKmsMrkDiscoveryKeyringInput = CreateAwsKmsMrkDiscoveryKeyringInput ( nameonly kmsClient: ComAmazonawsKmsTypes.IKeyManagementServiceClient ,
+ nameonly grantTokens: Option<GrantTokenList>
+ )
+ datatype CreateAwsKmsMrkDiscoveryKeyringInput = | CreateAwsKmsMrkDiscoveryKeyringInput (
+ nameonly kmsClient: ComAmazonawsKmsTypes.IKeyManagementServiceClient ,
  nameonly discoveryFilter: Option<DiscoveryFilter> ,
  nameonly grantTokens: Option<GrantTokenList> ,
- nameonly region: Region )
- datatype CreateAwsKmsMrkDiscoveryMultiKeyringInput = CreateAwsKmsMrkDiscoveryMultiKeyringInput ( nameonly regions: RegionList ,
+ nameonly region: Region
+ )
+ datatype CreateAwsKmsMrkDiscoveryMultiKeyringInput = | CreateAwsKmsMrkDiscoveryMultiKeyringInput (
+ nameonly regions: RegionList ,
  nameonly discoveryFilter: Option<DiscoveryFilter> ,
  nameonly clientSupplier: Option<IClientSupplier> ,
- nameonly grantTokens: Option<GrantTokenList> )
- datatype CreateAwsKmsMrkKeyringInput = CreateAwsKmsMrkKeyringInput ( nameonly kmsKeyId: KmsKeyId ,
+ nameonly grantTokens: Option<GrantTokenList>
+ )
+ datatype CreateAwsKmsMrkKeyringInput = | CreateAwsKmsMrkKeyringInput (
+ nameonly kmsKeyId: KmsKeyId ,
  nameonly kmsClient: ComAmazonawsKmsTypes.IKeyManagementServiceClient ,
- nameonly grantTokens: Option<GrantTokenList> )
- datatype CreateAwsKmsMrkMultiKeyringInput = CreateAwsKmsMrkMultiKeyringInput ( nameonly generator: Option<KmsKeyId> ,
+ nameonly grantTokens: Option<GrantTokenList>
+ )
+ datatype CreateAwsKmsMrkMultiKeyringInput = | CreateAwsKmsMrkMultiKeyringInput (
+ nameonly generator: Option<KmsKeyId> ,
  nameonly kmsKeyIds: Option<KmsKeyIdList> ,
  nameonly clientSupplier: Option<IClientSupplier> ,
- nameonly grantTokens: Option<GrantTokenList> )
- datatype CreateAwsKmsMultiKeyringInput = CreateAwsKmsMultiKeyringInput ( nameonly generator: Option<KmsKeyId> ,
+ nameonly grantTokens: Option<GrantTokenList>
+ )
+ datatype CreateAwsKmsMultiKeyringInput = | CreateAwsKmsMultiKeyringInput (
+ nameonly generator: Option<KmsKeyId> ,
  nameonly kmsKeyIds: Option<KmsKeyIdList> ,
  nameonly clientSupplier: Option<IClientSupplier> ,
- nameonly grantTokens: Option<GrantTokenList> )
- datatype CreateDefaultClientSupplierInput = CreateDefaultClientSupplierInput (  )
- datatype CreateDefaultCryptographicMaterialsManagerInput = CreateDefaultCryptographicMaterialsManagerInput ( nameonly keyring: IKeyring )
- datatype CreateMultiKeyringInput = CreateMultiKeyringInput ( nameonly generator: Option<IKeyring> ,
- nameonly childKeyrings: KeyringList )
- datatype CreateRawAesKeyringInput = CreateRawAesKeyringInput ( nameonly keyNamespace: string ,
+ nameonly grantTokens: Option<GrantTokenList>
+ )
+ datatype CreateDefaultClientSupplierInput = | CreateDefaultClientSupplierInput (
+ 
+ )
+ datatype CreateDefaultCryptographicMaterialsManagerInput = | CreateDefaultCryptographicMaterialsManagerInput (
+ nameonly keyring: IKeyring
+ )
+ datatype CreateMultiKeyringInput = | CreateMultiKeyringInput (
+ nameonly generator: Option<IKeyring> ,
+ nameonly childKeyrings: KeyringList
+ )
+ datatype CreateRawAesKeyringInput = | CreateRawAesKeyringInput (
+ nameonly keyNamespace: string ,
  nameonly keyName: string ,
  nameonly wrappingKey: seq<uint8> ,
- nameonly wrappingAlg: AesWrappingAlg )
- datatype CreateRawRsaKeyringInput = CreateRawRsaKeyringInput ( nameonly keyNamespace: string ,
+ nameonly wrappingAlg: AesWrappingAlg
+ )
+ datatype CreateRawRsaKeyringInput = | CreateRawRsaKeyringInput (
+ nameonly keyNamespace: string ,
  nameonly keyName: string ,
  nameonly paddingScheme: PaddingScheme ,
  nameonly publicKey: Option<seq<uint8>> ,
- nameonly privateKey: Option<seq<uint8>> )
- trait {:termination false} ICryptographicMaterialsManager {
- predicate {:opaque} GetEncryptionMaterialsCalledWith ( input: GetEncryptionMaterialsInput ) {true}
- predicate {:opaque} GetEncryptionMaterialsSucceededWith (  input: GetEncryptionMaterialsInput , output: GetEncryptionMaterialsOutput ) {true}
- method GetEncryptionMaterials ( input: GetEncryptionMaterialsInput ) returns  ( output: Result<GetEncryptionMaterialsOutput, Error> )
+ nameonly privateKey: Option<seq<uint8>>
+ )
+ trait {:termination false} ICryptographicMaterialsManager
+ {
+ method GetEncryptionMaterials ( input: GetEncryptionMaterialsInput ) returns (output: Result<GetEncryptionMaterialsOutput, Error>)
 	ensures GetEncryptionMaterialsCalledWith (  input )
 	ensures output.Success? ==> GetEncryptionMaterialsSucceededWith (  input , output.value )
-
- predicate {:opaque} DecryptMaterialsCalledWith ( input: DecryptMaterialsInput ) {true}
- predicate {:opaque} DecryptMaterialsSucceededWith (  input: DecryptMaterialsInput , output: DecryptMaterialsOutput ) {true}
- method DecryptMaterials ( input: DecryptMaterialsInput ) returns  ( output: Result<DecryptMaterialsOutput, Error> )
+ method DecryptMaterials ( input: DecryptMaterialsInput ) returns (output: Result<DecryptMaterialsOutput, Error>)
 	ensures DecryptMaterialsCalledWith (  input )
 	ensures output.Success? ==> DecryptMaterialsSucceededWith (  input , output.value )
-
 }
- datatype DecryptionMaterials = DecryptionMaterials ( nameonly algorithmSuiteId: AlgorithmSuiteId ,
+ // Predicates are separated from the trait. This is temporary.
+ predicate {:opaque} GetEncryptionMaterialsCalledWith ( input: GetEncryptionMaterialsInput ) {true}
+ predicate {:opaque} GetEncryptionMaterialsSucceededWith (  input: GetEncryptionMaterialsInput , output: GetEncryptionMaterialsOutput ) {true}
+ predicate {:opaque} DecryptMaterialsCalledWith ( input: DecryptMaterialsInput ) {true}
+ predicate {:opaque} DecryptMaterialsSucceededWith (  input: DecryptMaterialsInput , output: DecryptMaterialsOutput ) {true}
+ datatype DecryptionMaterials = | DecryptionMaterials (
+ nameonly algorithmSuite: AlgorithmSuiteInfo ,
  nameonly encryptionContext: EncryptionContext ,
  nameonly plaintextDataKey: Option<seq<uint8>> ,
- nameonly verificationKey: Option<seq<uint8>> )
- datatype DecryptMaterialsInput = DecryptMaterialsInput ( nameonly algorithmSuiteId: AlgorithmSuiteId ,
+ nameonly verificationKey: Option<seq<uint8>>
+ )
+ datatype DecryptMaterialsInput = | DecryptMaterialsInput (
+ nameonly algorithmSuiteId: AlgorithmSuiteId ,
  nameonly commitmentPolicy: CommitmentPolicy ,
  nameonly encryptedDataKeys: EncryptedDataKeyList ,
- nameonly encryptionContext: EncryptionContext )
- datatype DecryptMaterialsOutput = DecryptMaterialsOutput ( nameonly decryptionMaterials: DecryptionMaterials )
+ nameonly encryptionContext: EncryptionContext
+ )
+ datatype DecryptMaterialsOutput = | DecryptMaterialsOutput (
+ nameonly decryptionMaterials: DecryptionMaterials
+ )
  datatype DerivationAlgorithm =
- | HKDF ( nameonly hmac: AwsCryptographyPrimitivesTypes.DigestAlgorithm ,
- nameonly saltLength: AwsCryptographyPrimitivesTypes.PositiveInteger ,
- nameonly inputKeyLength: AwsCryptographyPrimitivesTypes.PositiveInteger ,
- nameonly outputKeyLength: AwsCryptographyPrimitivesTypes.PositiveInteger )
- | IDENTITY (  )
- | None (  )
- datatype DiscoveryFilter = DiscoveryFilter ( nameonly accountIds: AccountIdList ,
- nameonly partition: string )
- datatype EncryptedDataKey = EncryptedDataKey ( nameonly keyProviderId: Utf8Bytes ,
+ | HKDF(HKDF: HKDF)
+ | IDENTITY(IDENTITY: IDENTITY)
+ | None(None: None)
+ datatype DiscoveryFilter = | DiscoveryFilter (
+ nameonly accountIds: AccountIdList ,
+ nameonly partition: string
+ )
+ datatype ECDSA = | ECDSA (
+ nameonly curve: string
+ )
+ datatype EncryptedDataKey = | EncryptedDataKey (
+ nameonly keyProviderId: Utf8Bytes ,
  nameonly keyProviderInfo: seq<uint8> ,
- nameonly ciphertext: seq<uint8> )
+ nameonly ciphertext: seq<uint8>
+ )
  type EncryptedDataKeyList = seq<EncryptedDataKey>
  type EncryptionContext = map<Utf8Bytes, Utf8Bytes>
- datatype EncryptionMaterials = EncryptionMaterials ( nameonly algorithmSuiteId: AlgorithmSuiteId ,
+ datatype EncryptionMaterials = | EncryptionMaterials (
+ nameonly algorithmSuite: AlgorithmSuiteInfo ,
  nameonly encryptionContext: EncryptionContext ,
  nameonly encryptedDataKeys: EncryptedDataKeyList ,
  nameonly plaintextDataKey: Option<seq<uint8>> ,
- nameonly signingKey: Option<seq<uint8>> )
- datatype GetClientInput = GetClientInput ( nameonly region: Region )
- datatype GetEncryptionMaterialsInput = GetEncryptionMaterialsInput ( nameonly encryptionContext: EncryptionContext ,
+ nameonly signingKey: Option<seq<uint8>>
+ )
+ datatype GetClientInput = | GetClientInput (
+ nameonly region: Region
+ )
+ datatype GetEncryptionMaterialsInput = | GetEncryptionMaterialsInput (
+ nameonly encryptionContext: EncryptionContext ,
  nameonly commitmentPolicy: CommitmentPolicy ,
  nameonly algorithmSuiteId: Option<AlgorithmSuiteId> ,
- nameonly maxPlaintextLength: Option<int64> )
- datatype GetEncryptionMaterialsOutput = GetEncryptionMaterialsOutput ( nameonly encryptionMaterials: EncryptionMaterials )
+ nameonly maxPlaintextLength: Option<int64>
+ )
+ datatype GetEncryptionMaterialsOutput = | GetEncryptionMaterialsOutput (
+ nameonly encryptionMaterials: EncryptionMaterials
+ )
  type GrantTokenList = seq<string>
+ datatype HKDF = | HKDF (
+ nameonly hmac: AwsCryptographyPrimitivesTypes.DigestAlgorithm ,
+ nameonly saltLength: AwsCryptographyPrimitivesTypes.PositiveInteger ,
+ nameonly inputKeyLength: AwsCryptographyPrimitivesTypes.PositiveInteger ,
+ nameonly outputKeyLength: AwsCryptographyPrimitivesTypes.PositiveInteger
+ )
+ datatype IDENTITY = | IDENTITY (
+ 
+ )
+ datatype InitializeMaterialsInput = | InitializeMaterialsInput (
+ nameonly algorithmSuiteId: AlgorithmSuiteId ,
+ nameonly encryptionContext: EncryptionContext ,
+ nameonly signingKey: Option<seq<uint8>>
+ )
  type KeyringList = seq<IKeyring>
- trait {:termination false} IKeyring {
- predicate {:opaque} OnEncryptCalledWith ( input: OnEncryptInput ) {true}
- predicate {:opaque} OnEncryptSucceededWith (  input: OnEncryptInput , output: OnEncryptOutput ) {true}
- method OnEncrypt ( input: OnEncryptInput ) returns  ( output: Result<OnEncryptOutput, Error> )
+ trait {:termination false} IKeyring
+ {
+ method OnEncrypt ( input: OnEncryptInput ) returns (output: Result<OnEncryptOutput, Error>)
 	ensures OnEncryptCalledWith (  input )
 	ensures output.Success? ==> OnEncryptSucceededWith (  input , output.value )
-
- predicate {:opaque} OnDecryptCalledWith ( input: OnDecryptInput ) {true}
- predicate {:opaque} OnDecryptSucceededWith (  input: OnDecryptInput , output: OnDecryptOutput ) {true}
- method OnDecrypt ( input: OnDecryptInput ) returns  ( output: Result<OnDecryptOutput, Error> )
+ method OnDecrypt ( input: OnDecryptInput ) returns (output: Result<OnDecryptOutput, Error>)
 	ensures OnDecryptCalledWith (  input )
 	ensures output.Success? ==> OnDecryptSucceededWith (  input , output.value )
-
 }
+ // Predicates are separated from the trait. This is temporary.
+ predicate {:opaque} OnEncryptCalledWith ( input: OnEncryptInput ) {true}
+ predicate {:opaque} OnEncryptSucceededWith (  input: OnEncryptInput , output: OnEncryptOutput ) {true}
+ predicate {:opaque} OnDecryptCalledWith ( input: OnDecryptInput ) {true}
+ predicate {:opaque} OnDecryptSucceededWith (  input: OnDecryptInput , output: OnDecryptOutput ) {true}
  type KmsKeyId = string
  type KmsKeyIdList = seq<KmsKeyId>
- datatype MaterialProvidersConfig = MaterialProvidersConfig (  )
- datatype OnDecryptInput = OnDecryptInput ( nameonly materials: DecryptionMaterials ,
- nameonly encryptedDataKeys: EncryptedDataKeyList )
- datatype OnDecryptOutput = OnDecryptOutput ( nameonly materials: DecryptionMaterials )
- datatype OnEncryptInput = OnEncryptInput ( nameonly materials: EncryptionMaterials )
- datatype OnEncryptOutput = OnEncryptOutput ( nameonly materials: EncryptionMaterials )
+ datatype MaterialProvidersConfig = | MaterialProvidersConfig (
+ 
+ )
+ datatype None = | None (
+ 
+ )
+ datatype OnDecryptInput = | OnDecryptInput (
+ nameonly materials: DecryptionMaterials ,
+ nameonly encryptedDataKeys: EncryptedDataKeyList
+ )
+ datatype OnDecryptOutput = | OnDecryptOutput (
+ nameonly materials: DecryptionMaterials
+ )
+ datatype OnEncryptInput = | OnEncryptInput (
+ nameonly materials: EncryptionMaterials
+ )
+ datatype OnEncryptOutput = | OnEncryptOutput (
+ nameonly materials: EncryptionMaterials
+ )
  datatype PaddingScheme =
 	| PKCS1
 	| OAEP_SHA1_MGF1
@@ -247,14 +332,37 @@ include "../../StandardLibrary/StandardLibrary.dfy"
 	| OAEP_SHA512_MGF1
  type Region = string
  type RegionList = seq<Region>
+ datatype SignatureAlgorithm =
+ | ECDSA(ECDSA: ECDSA)
+ | None(None: None)
  type Utf8Bytes = ValidUTF8Bytes
+ datatype ValidDecryptionMaterialsTransitionInput = | ValidDecryptionMaterialsTransitionInput (
+ nameonly start: Option<DecryptionMaterials> ,
+ nameonly stop: Option<DecryptionMaterials>
+ )
+ datatype ValidEncryptionMaterialsTransitionInput = | ValidEncryptionMaterialsTransitionInput (
+ nameonly start: Option<EncryptionMaterials> ,
+ nameonly stop: Option<EncryptionMaterials>
+ )
  datatype Error =
  // Local Error structures are listed here
- | AwsCryptographicMaterialProvidersException ( nameonly message: string )
+ | AwsCryptographicMaterialProvidersException (
+ nameonly message: string
+ )
  // Any dependent models are listed here
- | AwsCryptographyPrimitivesTypesError(err: AwsCryptographyPrimitivesTypes.Error)
- | ComAmazonawsKmsTypesError(err: ComAmazonawsKmsTypes.Error)
+ | AwsCryptographyPrimitives(AwsCryptographyPrimitives: AwsCryptographyPrimitivesTypes.Error)
+ | ComAmazonawsKms(ComAmazonawsKms: ComAmazonawsKmsTypes.Error)
  // The Opaque error, used for native, extern, wrapped or unknown errors
  | Opaque(obj: object)
  type OpaqueError = e: Error | e.Opaque? witness *
+}
+ abstract module AwsCryptographyMaterialProvidersAbstract
+ {
+ import opened Wrappers
+ import opened StandardLibrary.UInt
+ import opened UTF8
+ import opened Types = AwsCryptographyMaterialProvidersTypes
+ function method DefaultMaterialProvidersConfig(): MaterialProvidersConfig
+ method MaterialProviders(config: MaterialProvidersConfig := DefaultMaterialProvidersConfig())
+ returns (res: Result<IAwsCryptographicMaterialProvidersClient, Error>)
 }
