src/Crypto/Model/AwsCryptographyPrimitivesTypes.dfy
@@ -8,126 +8,133 @@ include "../../StandardLibrary/StandardLibrary.dfy"
  import opened Wrappers
  import opened StandardLibrary.UInt
  import opened UTF8
- datatype AES_GCM = AES_GCM (
-	nameonly keyLength: int32 ,
-	nameonly tagLength: int32 ,
-	nameonly ivLength: int32 )
- datatype AESDecryptInput = AESDecryptInput (
-	nameonly encAlg: AES_GCM ,
-	nameonly key: seq<uint8> ,
-	nameonly cipherTxt: seq<uint8> ,
-	nameonly authTag: seq<uint8> ,
-	nameonly iv: seq<uint8> ,
-	nameonly aad: seq<uint8> )
- datatype AESEncryptInput = AESEncryptInput (
-	nameonly encAlg: AES_GCM ,
-	nameonly iv: seq<uint8> ,
-	nameonly key: seq<uint8> ,
-	nameonly msg: seq<uint8> ,
-	nameonly aad: seq<uint8> )
- datatype AESEncryptOutput = AESEncryptOutput (
-	nameonly cipherText: seq<uint8> ,
-	nameonly authTag: seq<uint8> )
- trait {:termination false} IAwsCryptographicPrimitivesClient {
- predicate GenerateRandomBytesCalledWith ( input: GenerateRandomBytesInput ) {true}
- predicate GenerateRandomBytesSucceededWith (  input: GenerateRandomBytesInput , output: seq<uint8> ) {true}
- method GenerateRandomBytes ( input: GenerateRandomBytesInput ) returns  ( output: Result<seq<uint8>, Error> )
+ datatype AES_GCM = | AES_GCM (
+ nameonly keyLength: int32 ,
+ nameonly tagLength: int32 ,
+ nameonly ivLength: int32
+ )
+ datatype AESDecryptInput = | AESDecryptInput (
+ nameonly encAlg: AES_GCM ,
+ nameonly key: seq<uint8> ,
+ nameonly cipherTxt: seq<uint8> ,
+ nameonly authTag: seq<uint8> ,
+ nameonly iv: seq<uint8> ,
+ nameonly aad: seq<uint8>
+ )
+ datatype AESEncryptInput = | AESEncryptInput (
+ nameonly encAlg: AES_GCM ,
+ nameonly iv: seq<uint8> ,
+ nameonly key: seq<uint8> ,
+ nameonly msg: seq<uint8> ,
+ nameonly aad: seq<uint8>
+ )
+ datatype AESEncryptOutput = | AESEncryptOutput (
+ nameonly cipherText: seq<uint8> ,
+ nameonly authTag: seq<uint8>
+ )
+ trait {:termination false} IAwsCryptographicPrimitivesClient
+ {
+ method GenerateRandomBytes ( input: GenerateRandomBytesInput ) returns (output: Result<seq<uint8>, Error>)
 	ensures GenerateRandomBytesCalledWith (  input )
 	ensures output.Success? ==> GenerateRandomBytesSucceededWith (  input , output.value )
-
- predicate DigestCalledWith ( input: DigestInput ) {true}
- predicate DigestSucceededWith (  input: DigestInput , output: seq<uint8> ) {true}
- method Digest ( input: DigestInput ) returns  ( output: Result<seq<uint8>, Error> )
+ method Digest ( input: DigestInput ) returns (output: Result<seq<uint8>, Error>)
 	ensures DigestCalledWith (  input )
 	ensures output.Success? ==> DigestSucceededWith (  input , output.value )
-
- predicate HMacCalledWith ( input: HMacInput ) {true}
- predicate HMacSucceededWith (  input: HMacInput , output: seq<uint8> ) {true}
- method HMac ( input: HMacInput ) returns  ( output: Result<seq<uint8>, Error> )
+ method HMac ( input: HMacInput ) returns (output: Result<seq<uint8>, Error>)
 	ensures HMacCalledWith (  input )
 	ensures output.Success? ==> HMacSucceededWith (  input , output.value )
-
- predicate HkdfExtractCalledWith ( input: HkdfExtractInput ) {true}
- predicate HkdfExtractSucceededWith (  input: HkdfExtractInput , output: seq<uint8> ) {true}
- method HkdfExtract ( input: HkdfExtractInput ) returns  ( output: Result<seq<uint8>, Error> )
+ method HkdfExtract ( input: HkdfExtractInput ) returns (output: Result<seq<uint8>, Error>)
 	ensures HkdfExtractCalledWith (  input )
 	ensures output.Success? ==> HkdfExtractSucceededWith (  input , output.value )
-
- predicate HkdfExpandCalledWith ( input: HkdfExpandInput ) {true}
- predicate HkdfExpandSucceededWith (  input: HkdfExpandInput , output: seq<uint8> ) {true}
- method HkdfExpand ( input: HkdfExpandInput ) returns  ( output: Result<seq<uint8>, Error> )
+ method HkdfExpand ( input: HkdfExpandInput ) returns (output: Result<seq<uint8>, Error>)
 	ensures HkdfExpandCalledWith (  input )
 	ensures output.Success? ==> HkdfExpandSucceededWith (  input , output.value )
-
- predicate HkdfCalledWith ( input: HkdfInput ) {true}
- predicate HkdfSucceededWith (  input: HkdfInput , output: seq<uint8> ) {true}
- method Hkdf ( input: HkdfInput ) returns  ( output: Result<seq<uint8>, Error> )
+ method Hkdf ( input: HkdfInput ) returns (output: Result<seq<uint8>, Error>)
 	ensures HkdfCalledWith (  input )
 	ensures output.Success? ==> HkdfSucceededWith (  input , output.value )
-
- predicate AESEncryptCalledWith ( input: AESEncryptInput ) {true}
- predicate AESEncryptSucceededWith (  input: AESEncryptInput , output: AESEncryptOutput ) {true}
- method AESEncrypt ( input: AESEncryptInput ) returns  ( output: Result<AESEncryptOutput, Error> )
+ method AESEncrypt ( input: AESEncryptInput ) returns (output: Result<AESEncryptOutput, Error>)
 	ensures AESEncryptCalledWith (  input )
 	ensures output.Success? ==> AESEncryptSucceededWith (  input , output.value )
-
- predicate AESDecryptCalledWith ( input: AESDecryptInput ) {true}
- predicate AESDecryptSucceededWith (  input: AESDecryptInput , output: seq<uint8> ) {true}
- method AESDecrypt ( input: AESDecryptInput ) returns  ( output: Result<seq<uint8>, Error> )
+ method AESDecrypt ( input: AESDecryptInput ) returns (output: Result<seq<uint8>, Error>)
 	ensures AESDecryptCalledWith (  input )
 	ensures output.Success? ==> AESDecryptSucceededWith (  input , output.value )
-
 }
- datatype CryptoConfig = CryptoConfig (  )
+ // Predicates are separated from the trait. This is temporary.
+ predicate {:opaque} GenerateRandomBytesCalledWith ( input: GenerateRandomBytesInput ) {true}
+ predicate {:opaque} GenerateRandomBytesSucceededWith (  input: GenerateRandomBytesInput , output: seq<uint8> ) {true}
+ predicate {:opaque} DigestCalledWith ( input: DigestInput ) {true}
+ predicate {:opaque} DigestSucceededWith (  input: DigestInput , output: seq<uint8> ) {true}
+ predicate {:opaque} HMacCalledWith ( input: HMacInput ) {true}
+ predicate {:opaque} HMacSucceededWith (  input: HMacInput , output: seq<uint8> ) {true}
+ predicate {:opaque} HkdfExtractCalledWith ( input: HkdfExtractInput ) {true}
+ predicate {:opaque} HkdfExtractSucceededWith (  input: HkdfExtractInput , output: seq<uint8> ) {true}
+ predicate {:opaque} HkdfExpandCalledWith ( input: HkdfExpandInput ) {true}
+ predicate {:opaque} HkdfExpandSucceededWith (  input: HkdfExpandInput , output: seq<uint8> ) {true}
+ predicate {:opaque} HkdfCalledWith ( input: HkdfInput ) {true}
+ predicate {:opaque} HkdfSucceededWith (  input: HkdfInput , output: seq<uint8> ) {true}
+ predicate {:opaque} AESEncryptCalledWith ( input: AESEncryptInput ) {true}
+ predicate {:opaque} AESEncryptSucceededWith (  input: AESEncryptInput , output: AESEncryptOutput ) {true}
+ predicate {:opaque} AESDecryptCalledWith ( input: AESDecryptInput ) {true}
+ predicate {:opaque} AESDecryptSucceededWith (  input: AESDecryptInput , output: seq<uint8> ) {true}
+ datatype CryptoConfig = | CryptoConfig (
+ 
+ )
  datatype DigestAlgorithm =
 	| SHA_512
 	| SHA_384
 	| SHA_256
- datatype DigestInput = DigestInput (
-	nameonly digestAlgorithm: DigestAlgorithm ,
-	nameonly message: seq<uint8> )
- datatype GenerateRandomBytesInput = GenerateRandomBytesInput (
-	nameonly length: int32 )
- datatype HkdfExpandInput = HkdfExpandInput (
-	nameonly digestAlgorithm: DigestAlgorithm ,
-	nameonly prk: seq<uint8> ,
-	nameonly info: Option<seq<uint8>> ,
-	nameonly expectedLength: int32 )
- datatype HkdfExtractInput = HkdfExtractInput (
-	nameonly digest: DigestAlgorithm ,
-	nameonly salt: Option<seq<uint8>> ,
-	nameonly ikm: seq<uint8> )
- datatype HkdfInput = HkdfInput (
-	nameonly digest: DigestAlgorithm ,
-	nameonly salt: Option<seq<uint8>> ,
-	nameonly ikm: seq<uint8> ,
-	nameonly info: Option<seq<uint8>> ,
-	nameonly expectedLength: int64 )
- datatype HMacInput = HMacInput (
-	nameonly digestAlgorithm: DigestAlgorithm ,
-	nameonly key: seq<uint8> ,
-	nameonly message: seq<uint8> )
- type UnsignedInteger = x: int32 | IsValid_UnsignedInteger(x) witness *
- predicate method IsValid_UnsignedInteger(x: int32) {
+ datatype DigestInput = | DigestInput (
+ nameonly digestAlgorithm: DigestAlgorithm ,
+ nameonly message: seq<uint8>
+ )
+ datatype GenerateRandomBytesInput = | GenerateRandomBytesInput (
+ nameonly length: int32
+ )
+ datatype HkdfExpandInput = | HkdfExpandInput (
+ nameonly digestAlgorithm: DigestAlgorithm ,
+ nameonly prk: seq<uint8> ,
+ nameonly info: Option<seq<uint8>> ,
+ nameonly expectedLength: int32
+ )
+ datatype HkdfExtractInput = | HkdfExtractInput (
+ nameonly digest: DigestAlgorithm ,
+ nameonly salt: Option<seq<uint8>> ,
+ nameonly ikm: seq<uint8>
+ )
+ datatype HkdfInput = | HkdfInput (
+ nameonly digest: DigestAlgorithm ,
+ nameonly salt: Option<seq<uint8>> ,
+ nameonly ikm: seq<uint8> ,
+ nameonly info: Option<seq<uint8>> ,
+ nameonly expectedLength: int64
+ )
+ datatype HMacInput = | HMacInput (
+ nameonly digestAlgorithm: DigestAlgorithm ,
+ nameonly key: seq<uint8> ,
+ nameonly message: seq<uint8>
+ )
+ type PositiveInteger = x: int32 | IsValid_PositiveInteger(x) witness *
+ predicate method IsValid_PositiveInteger(x: int32) {
  ( 0 <= x  )
 }
  datatype Error =
  // Local Error structures are listed here
  | AwsCryptographicPrimitivesError (
-	nameonly message: string )
+ nameonly message: string
+ )
  // Any dependent models are listed here
  
  // The Opaque error, used for native, extern, wrapped or unknown errors
  | Opaque(obj: object)
  type OpaqueError = e: Error | e.Opaque? witness *
 }
-
-abstract module AwsCryptographyPrimitivesService {
-	import opened Types = AwsCryptographyPrimitivesTypes
-	import opened Wrappers
-  import opened StandardLibrary.UInt
-
-	method AtomicPrimitives(config: CryptoConfig)
-		returns (res: Result<IAwsCryptographicPrimitivesClient,Error>)
-
+ abstract module AwsCryptographyPrimitivesAbstract
+ {
+ import opened Wrappers
+ import opened StandardLibrary.UInt
+ import opened UTF8
+ import opened Types = AwsCryptographyPrimitivesTypes
+ function method DefaultCryptoConfig(): CryptoConfig
+ method Crypto(config: CryptoConfig := DefaultCryptoConfig())
+ returns (res: Result<IAwsCryptographicPrimitivesClient, Error>)
 }
