src/SDK/Model/AwsEncryptionSdkTypes.dfy
@@ -1,0 +1,68 @@
+// Copyright Amazon.com Inc. or its affiliates. All Rights Reserved.
+// SPDX-License-Identifier: Apache-2.0
+// Do not modify this file. This file is machine generated, and any changes to it will be overwritten.
+include "../../StandardLibrary/StandardLibrary.dfy"
+ include "../../Util/UTF8.dfy"
+ include "../../AwsCryptographicMaterialProviders/Model/AwsCryptographyMaterialProvidersTypes.dfy"
+ module AwsEncryptionSdkTypes
+ {
+ import opened Wrappers
+ import opened StandardLibrary.UInt
+ import opened UTF8
+ import AwsCryptographyMaterialProvidersTypes
+ trait {:termination false} IAwsEncryptionSdkClient {
+ predicate {:opaque} EncryptCalledWith ( input: EncryptInput ) {true}
+ predicate {:opaque} EncryptSucceededWith (  input: EncryptInput , output: EncryptOutput ) {true}
+ method Encrypt ( input: EncryptInput ) returns  ( output: Result<EncryptOutput, Error> )
+	ensures EncryptCalledWith (  input )
+	ensures output.Success? ==> EncryptSucceededWith (  input , output.value )
+
+ predicate {:opaque} DecryptCalledWith ( input: DecryptInput ) {true}
+ predicate {:opaque} DecryptSucceededWith (  input: DecryptInput , output: DecryptOutput ) {true}
+ method Decrypt ( input: DecryptInput ) returns  ( output: Result<DecryptOutput, Error> )
+	ensures DecryptCalledWith (  input )
+	ensures output.Success? ==> DecryptSucceededWith (  input , output.value )
+
+}
+ datatype AwsEncryptionSdkConfig = | AwsEncryptionSdkConfig (
+ nameonly commitmentPolicy: Option<AwsCryptographyMaterialProvidersTypes.CommitmentPolicy> ,
+ nameonly maxEncryptedDataKeys: Option<CountingNumbers>
+ )
+ type CountingNumbers = x: int64 | IsValid_CountingNumbers(x) witness *
+ predicate method IsValid_CountingNumbers(x: int64) {
+ ( 1 <= x  )
+}
+ datatype DecryptInput = | DecryptInput (
+ nameonly ciphertext: seq<uint8> ,
+ nameonly materialsManager: Option<AwsCryptographyMaterialProvidersTypes.ICryptographicMaterialsManager> ,
+ nameonly keyring: Option<AwsCryptographyMaterialProvidersTypes.IKeyring>
+ )
+ datatype DecryptOutput = | DecryptOutput (
+ nameonly plaintext: seq<uint8> ,
+ nameonly encryptionContext: AwsCryptographyMaterialProvidersTypes.EncryptionContext ,
+ nameonly algorithmSuiteId: AwsCryptographyMaterialProvidersTypes.AlgorithmSuiteId
+ )
+ datatype EncryptInput = | EncryptInput (
+ nameonly plaintext: seq<uint8> ,
+ nameonly encryptionContext: Option<AwsCryptographyMaterialProvidersTypes.EncryptionContext> ,
+ nameonly materialsManager: Option<AwsCryptographyMaterialProvidersTypes.ICryptographicMaterialsManager> ,
+ nameonly keyring: Option<AwsCryptographyMaterialProvidersTypes.IKeyring> ,
+ nameonly algorithmSuiteId: Option<AwsCryptographyMaterialProvidersTypes.AlgorithmSuiteId> ,
+ nameonly frameLength: Option<int64>
+ )
+ datatype EncryptOutput = | EncryptOutput (
+ nameonly ciphertext: seq<uint8> ,
+ nameonly encryptionContext: AwsCryptographyMaterialProvidersTypes.EncryptionContext ,
+ nameonly algorithmSuiteId: AwsCryptographyMaterialProvidersTypes.AlgorithmSuiteId
+ )
+ datatype Error =
+ // Local Error structures are listed here
+ | AwsEncryptionSdkException (
+ nameonly message: string
+ )
+ // Any dependent models are listed here
+ | AwsCryptographyMaterialProviders(awsCryptographyMaterialProviders: AwsCryptographyMaterialProvidersTypes.Error)
+ // The Opaque error, used for native, extern, wrapped or unknown errors
+ | Opaque(obj: object)
+ type OpaqueError = e: Error | e.Opaque? witness *
+}
