src/AwsCryptographicMaterialProviders/Model/materials.smithy
@@ -1,0 +1,53 @@
+namespace aws.cryptography.materialProviders
+
+operation InitializeEncryptionMaterials {
+  input: InitializeMaterialsInput,
+  output: EncryptionMaterials,
+}
+
+operation InitializeDecryptionMaterials {
+  input: InitializeMaterialsInput,
+  output: DecryptionMaterials,
+}
+
+// The initilize input is the same
+// for both Encryption and Dedryption materials.
+// This is because they MUST match.
+// The the Decryption materials did not
+// have exactly the same encryptoion context, for example 
+// then decryption should fail.
+structure InitializeMaterialsInput {
+  @required
+  algorithmSuiteId: AlgorithmSuiteId,
+
+  @required
+  encryptionContext: EncryptionContext,
+
+  @sensitive
+  signingKey: Blob
+}
+
+operation ValidEncryptionMaterialsTransition {
+  input: ValidEncryptionMaterialsTransitionInput,
+  output: ValidTransition
+}
+
+operation ValidDecryptionMaterialsTransition {
+  input: ValidDecryptionMaterialsTransitionInput,
+  output: ValidTransition
+}
+
+structure ValidEncryptionMaterialsTransitionInput {
+  start: EncryptionMaterials,
+  stop: EncryptionMaterials,
+}
+
+structure ValidDecryptionMaterialsTransitionInput {
+  start: DecryptionMaterials,
+  stop: DecryptionMaterials,
+}
+
+@aws.polymorph#positional
+structure ValidTransition {
+  valid: Boolean
+}
